Fifteen/Data/Array/Basic.lean
@@ -15,17 +15,47 @@ import Fifteen.Data.List.Basic
 -- Disable auto-binding of unbounded variables
 set_option autoImplicit false
 
-universe u
+universe u v
 
 namespace Array
 
 variable {α : Type u}
+
+/--
+:::note warn
+This theorem depends on `Classical.choice` since `Array.append_data` does.
+:::
+-/
+theorem size_append (as bs : Array α) : (as ++ bs).size = as.size + bs.size := by
+  dsimp [size]; rw [append_data, List.length_append]
 
 theorem getElem_swap (as : Array α) (i j : Fin as.size) (k : Nat) {hk : k < (as.swap i j).size} : (as.swap i j)[k] = if j.1 = k then as[i.1] else if i.1 = k then as[j.1] else as[k]'(as.size_swap i j ▸ hk) := by
   have : ∀ {m n : Nat} (h : m = n) (i : Fin m), ((h ▸ i) : Fin n).val = i.val :=
     @fun
     | _, _, rfl, _ => rfl
   simp [swap, getElem_eq_data_get, List.get_set, this]
+
+/--
+:::note warn
+This theorem depends on `Classical.choice` since `Array.append_data` does.
+:::
+-/
+theorem getElem_append_left {i : Nat} (as bs : Array α) (h : i < as.size) {h' : i < (as ++ bs).size} : (as ++ bs)[i] = as[i] := by
+  rewrite [getElem_eq_data_get]
+  rewrite [List.get_of_eq (Array.append_data as bs)]
+  rewrite [List.get_append_left as.data bs.data h]
+  rfl
+
+/--
+:::note warn
+This theorem depends on `Classical.choice` since `Array.append_data` does.
+:::
+-/
+theorem getElem_append_right {i : Nat} (as bs : Array α) (h : i ≥ as.size) {h' : i < (as ++ bs).size} : (as ++ bs)[i] = bs[i-as.size]'(Nat.sub_lt_left_of_lt_add h (Array.size_append as bs ▸ h')) := by
+  rewrite [getElem_eq_data_get]
+  rewrite [List.get_of_eq (Array.append_data as bs)]
+  rewrite [List.get_append_right' h]
+  rfl
 
 /-- The counterpart of `List.Nodup` in `Std` -/
 def Nodup (as : Array α) : Prop :=
@@ -48,6 +78,54 @@ theorem nodup_of_get_inj (as : Array α) (h : ∀ (i j : Nat) (hi : i < as.size)
 
 theorem Nodup.get_inj {as : Array α} (h : as.Nodup) (i j : Nat) (hi : i < as.size) (hj : j < as.size) : as[i] = as[j] → i = j :=
   List.Nodup.get_inj h (hi:=hi) (hj:=hj)
+
+/--
+:::note warn
+The lemma depends on `Classical.choice` since `Array.getElem_append_left`, `Array.getElem_append_right`, and etc do.
+:::
+-/
+theorem nodup_append {as bs : Array α} (has : as.Nodup) (hbs : bs.Nodup) (hdisj : ∀ (i j : Nat) (hi : i < as.size) (hj : j < bs.size), as[i] ≠ bs[j]) : (as ++ bs).Nodup :=
+  nodup_of_get_inj _ fun i j hi hj => by
+    if hi' : i < as.size then
+      rewrite [getElem_append_left as bs hi']
+      if hj' : j < as.size then
+        rewrite [getElem_append_left as bs hj']
+        exact has.get_inj i j hi' hj'
+      else
+        rewrite [getElem_append_right as bs (Nat.le_of_not_lt hj')]
+        intro hij; exfalso
+        exact hdisj _ _ _ _ hij
+    else
+      have hi'' : i ≥ as.size := Nat.le_of_not_lt hi'
+      have : i - as.size < bs.size :=
+        Nat.sub_lt_left_of_lt_add hi'' (size_append _ _ ▸ hi)
+      rewrite [getElem_append_right as bs (Nat.le_of_not_lt hi')]
+      if hj' : j < as.size then
+        rewrite [getElem_append_left as bs hj']
+        intro hij; exfalso
+        exact hdisj _ _ _ _ hij.symm
+      else
+        have hj'' : j ≥ as.size := Nat.le_of_not_lt hj'
+        have : j - as.size < bs.size :=
+          Nat.sub_lt_left_of_lt_add hj'' (size_append _ _ ▸ hj)
+        rewrite [getElem_append_right as bs (Nat.le_of_not_lt hj')]
+        intro h
+        have := hbs.get_inj (i-as.size) (j-as.size) ‹_› ‹_› h
+        conv at this =>
+          rewrite [Nat.sub_eq_iff_eq_add hi'']
+          rewrite [Nat.sub_add_cancel hj'']
+        exact this
+
+/--
+:::note warn
+The lemma depends on `Classical.choice` since `Array.getElem_map` does.
+:::
+-/
+theorem nodup_map {β : Type v} (f : α → β) (as : Array α) (has : as.Nodup) (hf : ∀ a₁ a₂, f a₁ = f a₂ → a₁ = a₂) : (as.map f).Nodup :=
+  nodup_of_get_inj _ fun i j hi hj h => by
+    conv at h =>
+      simp only [Array.getElem_map]
+    apply has.get_inj; apply hf _ _ h
 
 theorem nodup_swap (as : Array α) (i j : Fin as.size) (h : as.Nodup) : (as.swap i j).Nodup := by
   apply nodup_of_get_inj; intro k l hk hl has
